\documentclass[11pt]{homework}

% TODO: replace these with your information
\newcommand{\hwname}{ZHOU Yuming}
\newcommand{\hwemail}{\href{mailto://121050081@link.cuhk.edu.cn}{121050081@link.cuhk.edu.cn}}
\newcommand{\hwtype}{Homework}
\newcommand{\hwnum}{1}
\newcommand{\hwclass}{MAT2040-T13}
\newcommand{\hwlecture}{0}
\newcommand{\hwsection}{Z}

\input{preamble}

\begin{document}
\maketitle

% Your content
    \question
    \begin{arabicparts}
        \questionpart
            \begin{equation}
                A= 
                \begin{bmatrix}
                1 & 2 & 1 \\
                -1 & 1 & 2\\
                1 & 1 & -1
                \end{bmatrix}
            \end{equation}
            \begin{equation}
                B= 
                \begin{bmatrix}
                    3\\
                    2\\
                    1
                \end{bmatrix}
            \end{equation}
            \begin{equation}
                [A|b]=
                \left[\begin{array}{ccc|c}
                1 & 2 & 1 & 3 \\ 
                -1 & 1 & 2 & 2 \\ 
                1 & 1 & -1 & 1
                \end{array}\right]
            \end{equation} 
        \questionpart
            \begin{multline}
                [A|b]
                \rop{\Row{2}\to\Row{1}+\Row{2}\\\Row{3}\to-\Row{1}+\Row{3}}
                \left[\begin{array}{ccc|c}
                1 & 2 & 1 & 3 \\ 
                0 & 3 & 3 & 5 \\ 
                0 & -1 & -2 & -2
                \end{array}\right]
                \rop{\Row{3}\to3\Row{3}+\Row{2}}
                \left[\begin{array}{ccc|c}
                1 & 2 & 1 & 3 \\ 
                0 & 3 & 3 & 5 \\ 
                0 & 0 & -3 & -1
                \end{array}\right]\\
                \rop{\Row{3}\to-\frac{1}{3}\Row{3} }
                \left[\begin{array}{ccc|c}
                1 & 2 & 1 & 3 \\ 
                0 & 3 & 3 & 5 \\ 
                0 & 0 & 1 & \frac{1}{3}
                \end{array}\right]
                \rop{\Row{1}\to -\Row{3}+\Row{1}\\\Row{2}\to-3\Row{3}+\Row{2}}
                \left[\begin{array}{ccc|c}
                1 & 2 & 0 & \frac{8}{3} \\ 
                0 & 3 & 0 & 4 \\ 
                0 & 0 & 1 & \frac{1}{3}
                \end{array}\right]\\
                \rop{\Row{2}\to\frac{1}{3}\Row{2}\\\Row{1}\to-2\Row{2}+\Row{1}}
                \left[\begin{array}{ccc|c}
                1 & 0 & 0 & 0 \\ 
                0 & 1 & 0 & \frac{4}{3} \\ 
                0 & 0 & 1 & \frac{1}{3}
                \end{array}\right]
            \end{multline}
            \begin{equation}
                S=
                \left[\begin{array}{c}
                0 \\ 
                \frac{4}{3} \\ 
                \frac{1}{3}
                \end{array}\right]
            \end{equation}
    \end{arabicparts}
    \newpage
    \question
    \begin{multline}
        \left[\begin{array}{ccccc|c}
            4 & 5 & 3 & 3 & 4 & -5 \\ 
            2 & 3 & 1 & 0 & 1 & -3 \\ 
            3 & 4 & 2 & 1 & 2 & -1
            \end{array}\right]
        \rop{\Row{2}\to-\frac{1}{2}\Row{1}+\Row{2}\\\Row{3}\to-\frac{3}{4}\Row{1}+\Row{3}}
        \left[\begin{array}{ccccc|c}
        4 & 5 & 3 & 3 & 4 & -5 \\ 
        0 & \frac{1}{2} & -\frac{1}{2} & -\frac{1}{2} & -1 & -\frac{1}{2} \\ 
        0 & \frac{1}{4} & -\frac{1}{4} & -\frac{5}{4} & -1 & \frac{11}{4}
        \end{array}\right]\\
        \rop{\Row{2}\to2\Row{2}\\\Row{3}\to4\Row{3}\\\Row{3}\to\Row{3}-\Row{2}}
        \left[\begin{array}{ccccc|c}
        4 & 5 & 3 & 3 & 4 & -5 \\ 
        0 & 1 & -1 & -3 & -2 & -1 \\ 
        0 & 0 & 0 & -2 & -2 & 12
        \end{array}\right]
        \rop{\Row{3}\to-\frac{1}{2}\Row{3}\\
        \Row{2}\to\Row{2}+3\Row{3}\\
        \Row{1}\to\Row{1}-3\Row{3}}
        \left[\begin{array}{ccccc|c}
        4 & 5 & 3 & 0 & 1 & 13 \\ 
        0 & 1 & -1 & 0 & 1 & -19 \\ 
        0 & 0 & 0 & 1 & 1 & -6
        \end{array}\right]\\
        \rop{\Row{1}\to\Row{1}-5\Row{2}\\
        \Row{1}\to\frac{1}{4}\Row{1}}
        \left[\begin{array}{ccccc|c}
        1 & 0 & 2 & 0 & -1 & 27 \\ 
        0 & 1 & -1 & 0 & 1 & -19 \\ 
        0 & 0 & 0 & 1 & 1 & -6
        \end{array}\right]
    \end{multline}
    \begin{equation}
        S=
        \left[\begin{array}{c}
        -2\x{3}+\x{5}+27 \\ 
        \x{3}-\x{5}-19 \\ 
        \x{3} \\ 
        -\x{5}-6 \\ 
        \x{6}
        \end{array}\right]
    \end{equation}



    \question
    In this question, we could use partition matrix:
    \begin{equation}
        AB=
        \left[\begin{array}{cc|cc}
        1 & 0 & a & b \\ 
        0 & 1 & c & d
        \end{array}\right]
        \left[\begin{array}{cc}
        -a & -b \\ 
        -c & -d \\ 
        \hline
        1 & 0 \\ 
        0 & 1
        \end{array}\right]=
        \left[\begin{array}{cc}
        -a & -b \\ 
        -c & -d
        \end{array}\right]+
        \left[\begin{array}{cc}
        a & b \\ 
        c & d
        \end{array}\right]=
        \left[\begin{array}{cc}
        0 & 0 \\ 
        0 & 0
        \end{array}\right]
    \end{equation}
    \begin{equation}
        BA=
        \left[\begin{array}{cc}
        -a & -b \\ 
        -c & -d \\ 
        \hline
        0 & 0 \\ 
        -1 & 1
        \end{array}\right]
        \left[\begin{array}{cc|cc}
        1 & 0 & a & b \\ 
        0 & 1 & c & d
        \end{array}\right]=
        \left[\begin{array}{cccc}
        -a & -b & -a^2-bc & -ab-bd \\ 
        -c & -d & -ac-cd & -bc-d^2 \\ 
        1 & 0 & a & b \\ 
        0 & 1 & c & d
        \end{array}\right]
    \end{equation}
    
    \question
    \begin{arabicparts}
        \questionpart
        \begin{multline}
            A^2-B^2\\
            =A\cdot A+B\cdot B\\
            =\tp{A}\cdot\tp{A}-\tp{B}\cdot\tp{B}\\
            =\tp{A\cdot A}-\tp{B\cdot B}\\
            =\tp{(A^2)-(B^2)}
        \end{multline}
        , so it is symmetric.

        \questionpart
        Let $\LHS=(A+B)(A-B)$ and $\RHS=[(A+B)(A-B)]^T$, then
        \begin{equation}
            \RHS
            =(A-B)^T(A+B)^T
            =(A^T-B^T)(A^T-B^T)
            =(A-B)(A+B)
            \neq\LHS
        \end{equation}
        , so it is not symmetric.
        
        \questionpart
        Let $\LHS=ABA$ and $\RHS=(ABA)^T$, then
        \begin{equation}
            \RHS=(BA)^TA^T=A^TB^TA^T=ABA=\LHS
        \end{equation}
        , so it is symmetric.

        \questionpart
        Let $\LHS=ABAB$ and $\RHS=(ABAB)^T$, then
        \begin{equation}
            \RHS=(AB)^T(AB)^T=B^TA^TB^TA^T=BABA\neq\LHS
        \end{equation}  
        , so it is not symmetric.
    \end{arabicparts}

    \question
    \begin{arabicparts}
        \questionpart
    
    \includegraphics{h1q5s1.png}

    No solution.\\
    \questionpart
    \begin{equation}
        \begin{cases}
            2x+y&=2\\
            x-y&=2\\
            x&=\frac{4}{3}
        \end{cases}
    \end{equation}
        \includegraphics{h1q5s2.png}


    
    \end{arabicparts}
    \question
    \begin{equation}
        \left[\begin{array}{cccc}
        \hlight{a} & 1 & 3 & r \\ 
        a & a & 4 & s \\ 
        a & a & 2a & t
        \end{array}\right]
        \to
        \left[\begin{array}{cccc}
        \hlight{a} & 1 & 3 & r \\ 
        0 & a-1 & 1 & s-r \\ 
        0 & a-1 & 2a-3 & t-r
        \end{array}\right]
    \end{equation}
    when $a\neq0$, the elimination fails to give the pivot.
    \begin{equation}
        \left[\begin{array}{cccc}
            \hlight{a} & 1 & 3 & r \\ 
            0 & a-1 & 1 & s-r \\ 
            0 & a-1 & 2a-3 & t-r
            \end{array}\right]
        \to
        \left[\begin{array}{cccc}
        a & 1 & 3 & r \\ 
        0 & \hlight{a-1} & 1 & s-r \\ 
        0 & 0 & 2a-4 & t-s
        \end{array}\right]
    \end{equation}
    when $a\neq1$, the elimination fails to give the pivot.
    \begin{equation}
        \left[\begin{array}{cccc}
            a & 1 & 3 & r \\ 
            0 & a-1 & 1 & s-r \\ 
            0 & 0 & \hlight{2a-4} & t-s
            \end{array}\right]
    \end{equation}
    when $a\neq2$, the elimination fails to give the pivot.

    Hence,
    \begin{equation}
        a=\begin{cases}
            0\\
            1\\
            2
        \end{cases}
    \end{equation}

    \question
    By
    \begin{equation}
        ab^T=
        \left[\begin{array}{cccc}
        39 & 99 & 420 & 207 \\ 
        45 & 33 & 782 & 199 \\ 
        100 & 80 & 49 & 73 \\ 
        59 & 18 & 75 & 46
        \end{array}\right]
        =
        \left[\begin{array}{cccc}
        a_1 b_1 & a_1 b_2  & a_1 b_3  & a_1 b_4  \\ 
        a_2 b_1  & a_2 b_2  & a_2 b_3  & a_2 b_4  \\ 
        a_3 b_1  & a_3 b_2  & a_3 b_3  & a_3 b_4  \\ 
        a_4 b_1  & a_4 b_2  & a_4 b_3  & a_4 b_4 
        \end{array}\right]
    \end{equation}
    we could get
    \begin{equation}
        a^Tb=a_1 b_1 + a_2 b_2 + a_3 b_3 + a_4 b_4=39+33+49+46=167
    \end{equation}

    \question
    \begin{multline}
        A^3=(ab^T)^3=
        (\begin{bmatrix}
        1 \\ 
        2 \\ 
        3
        \end{bmatrix}
        \cdot
        \left[\begin{array}{ccc}
        1 & 1 & 0
        \end{array}\right]
        )^3=
        \left[\begin{array}{ccc}
        1 & 1 & 0 \\ 
        2 & 2 & 0 \\ 
        3 & 3 & 0
        \end{array}\right]^3\\
        =
        \left[\begin{array}{ccc}
        1 & 1 & 0 \\ 
        2 & 2 & 0 \\ 
        3 & 3 & 0
        \end{array}\right]
        \left[\begin{array}{ccc}
        3 & 3 & 0 \\ 
        6 & 6 & 0 \\ 
        9 & 9 & 0
        \end{array}\right]=
        \left[\begin{array}{ccc}
        9 & 9 & 0 \\ 
        18 & 18 & 0 \\ 
        27 & 27 & 0
        \end{array}\right]
    \end{multline}
    
    
    \question
    Given
    \begin{align}
        (I-xy^T)^{-1}&=(I+xy^T)\\
        (I-xy^T)(I-xy^T)^{-1}&=(I-xy^T)(I+xy^T)\\
        (I-xy^T)(I-xy^T)^{-1}&=I^2-xy^T+xy^T+(xy^T)^2\\
        I&=I+x(y^Tx)y^T\\
        0&=x(y^Tx)y^T\label{eq25}
        % x^Ty &=a_1 b_1 +a_2 b_2 + a_3 b_3 + a_4 b_4\\
        % y^Tx &=a_1 b_1 +a_2 b_2 + a_3 b_3 + a_4 b_4\\
        % x^Ty &=0
    \end{align}
    % , it follows that
    % \begin{equation}
    %     y^Tx=x^Ty=0
    % \end{equation}
    % By eq. (24),
    % it is not hard to find that
    % \begin{align}
    %     (I-xy^T)^{-1}&=(I+xy^T)\\
    %     ((I-xy^T)^{-1})^T&=((I+xy^T))^T
    % \end{align}
    if $y^Tx=0$, then \cref{eq25} is true. 
    \question
    \begin{equation}
        C^n=B^{-1}ABB^{-1}AB\dots B^{-1}ABB^{-1}AB=B^{-1}\underbrace{A\dots A}_{\text{n times}}B=B^{-1}A^nB
    \end{equation}
\end{document}

